lab4/Stack.dfy
@@ -1,0 +1,101 @@
+class Stack{
+
+    ghost var s:seq<int>;
+
+    // Abstract state
+    function AbsInv(): bool {true}
+
+    // Concrete state
+    var a:array<int>;
+    var size:int;
+
+    function RepInv(): bool
+    reads `size, `a
+    {
+        0 <= size <= a.Length
+    }
+
+    function Sound():bool
+    reads this, a
+    {
+        AbsInv() && 
+        RepInv() && 
+        size == |s| && forall k :: 0 <= k < size ==> s[k] == a[k]
+    }
+
+    
+    // ADT Code && Spec
+
+
+    function Empty(): bool
+    reads `s
+    {
+        s == []
+    }
+
+    constructor()
+    ensures Sound() && Empty()
+    {
+        a := new int[10];
+        size := 0;
+        s := [];
+    }
+
+    method push(x: int)
+    requires Sound() 
+    ensures Sound() && s == old(s) + [x]
+    modifies `a, a, `size, `s
+    {
+        resize();
+
+        a[size] := x;
+        size := size + 1;
+        s := s + [x];
+    }
+
+    method resize()
+    requires Sound()
+    ensures Sound()
+    ensures size < a.Length
+    modifies `a
+    {
+        if( size == a.Length) {
+            var b := new int[a.Length*2+1];
+            var i := 0;
+            while i < size
+            decreases size - i
+            invariant 0 <= i <= size
+            invariant forall k :: 0 <= k < i ==> s[k] == b[k]
+            modifies b
+            {
+                b[i] := a[i];
+                i := i +1;
+            }
+            a := b;
+        }
+    }
+    
+
+    method pop() returns (x: int)
+    requires AbsInv() && !Empty()
+    // ambos a mesma coisa mas o segundo muito mais simples
+    //ensures RepInv() && s == old(s)[0..|s|-1] && x == old(s)[|old(s)|-1]
+    ensures AbsInv() && s + [x] == old(s)
+
+    static method main(){
+        var stack:Stack := new Stack();
+
+        stack.push(0);
+        var v0 := stack.pop();
+
+        stack.push(1);
+        stack.push(2);
+
+        var v1 := stack.pop();
+        var v2 := stack.pop();
+        assert stack.s == [];
+        assert v1 == 2 && v2 == 1;
+
+       
+    }
+}
